## partial fractions
### simple fractions
2 / x-1   +   5 / x+4 = ?  
Common denominator  

2x + 8 + 5x - 5  /  (x-1)(x+4)  

=  7x+3  /  (x-1)(x+4)


> We can combine algebraic fractions by putting them over common denominator  
### Now we need to do it backwards. 

7x+3  /  (x-1)(x+4)   =   A/ (x-1) + B/(x+4)  
  
7x+3  =  A(x+4) + B(x-1)  
Now solve that for A and B  
2 options:  
* x values that remove an A or B.
* compare coeffieceenints of x.  

#### Option 1:
when x = 1 : 10 = 5A  **A=2**  
when x = -4 : -25 = -5B  **B=5**  

#### Option 2:
Multiply everything  out first:  
7x+*3*  =  A+B)x + *(4A-B)*  
A+B = 7  
4A-B = 3  
When solved for A and B, agrees with previous method.  


### Example 1.3.2 printed notes
2x-1  /  (2x+1(x-3)

2x-1  /  (2x+1(x-3)  =  F/ (2x+1) + G/(x-3)

2x-1 = F(x-3) + G(2x+1)

x=3 : 5 = 7G  **G = 5/7**

x = -1/2 : F = **4/7**

**So:**
4/ 7(2x+1) + 5/ (7x-3)


### Example 1.3.3 printed notes
10x+18 / (2x+3)(2x+3)

R/ (2x+3)  +  T/ (2x+3)(2x+3)

R(2x+3 / (2x+3)(2x+3)  +  T/ (2x+3)(2x+3)

*10x*+18  =  *R(2x+3)* + T

10x = 2Rx
R = 5
5(3) + T = 18
So T = 3
